TranslationCorrectness.v
@@ -28,15 +28,6 @@ Require Import Rustre.SynchronousNat.
      where a clock is active.
  *)
 
-Lemma pm_in_dec: forall A i m, PM.In (A:=A) i m \/ ~PM.In (A:=A) i m.
-Proof.
-  unfold PM.In, PM.MapsTo.
-  intros A i m.
-  case (PM.find i m).
-  eauto.
-  right; intro; destruct H; discriminate H.
-Qed.
-
 (** ** Predicates *)
 
 (**
@@ -146,42 +137,6 @@ Qed.
          and test it on the example programs in DataflowSyntax.v
 *)
 
-Lemma stmt_eval_translate_eqns_cons:
-  forall mems menv env menv' env' eq eqs,
-    stmt_eval menv env (translate_eqns mems (eq :: eqs)) (menv', env')
-    <->
-    (exists menv'' env'',
-        stmt_eval menv env (translate_eqns mems eqs) (menv'', env'')
-        /\ stmt_eval menv'' env'' (translate_eqn mems eq) (menv', env')).
-Proof. (* TODO: redo proof *)
-  split.
-  - intro H.
-    unfold translate_eqns in H.
-    simpl in H.
-    apply stmt_eval_fold_left_shift in H.
-    destruct H as [menv'' H].
-    destruct H as [env'' H].
-    exists menv''. exists env''.
-    destruct H as [H1 H2].
-    split. apply H1.
-    inversion_clear H2.
-    inversion H0.
-    rewrite <- H2.
-    rewrite <- H4.
-    apply H.
-  - intro H.
-    destruct H as [menv'' H].
-    destruct H as [env'' H].
-    destruct H as [H1 H2].
-    unfold translate_eqns.
-    simpl.
-    apply stmt_eval_fold_left_shift.
-    exists menv''. exists env''.
-    split. apply H1.
-    eapply Icomp. apply H2.
-    apply Iskip.
-Qed.
-
 Inductive Is_present_in (mems: PS.t) (menv: memoryEnv) (env: valueEnv)
   : clock -> Prop :=
 | IsCbase: Is_present_in mems menv env Cbase
@@ -227,6 +182,58 @@ Proof.
       (left; constructor; assumption) || right; inversion_clear 1; auto.
     + right; inversion_clear 1; auto.
 Qed.
+
+Lemma exp_eval_tovar:
+  forall x v menv env memories,
+    exp_eval menv env (tovar memories x) v
+    <-> (exp_eval menv env (State x) v /\ PS.In x memories)
+        \/ (exp_eval menv env (Var x) v /\ ~PS.In x memories).
+Proof.
+  split; intro Heval;
+  destruct In_dec with x memories as [Hxm|Hxm];
+    pose proof Hxm as Hxmt;
+    apply PS.mem_spec in Hxmt || apply mem_spec_false in Hxmt;
+    unfold tovar in *;
+    rewrite Hxmt in *;
+    intuition.
+Qed.
+
+Lemma stmt_eval_translate_eqns_cons:
+  forall mems menv env menv' env' eq eqs,
+    stmt_eval menv env (translate_eqns mems (eq :: eqs)) (menv', env')
+    <->
+    (exists menv'' env'',
+        stmt_eval menv env (translate_eqns mems eqs) (menv'', env'')
+        /\ stmt_eval menv'' env'' (translate_eqn mems eq) (menv', env')).
+Proof. (* TODO: redo proof *)
+  split.
+  - intro H.
+    unfold translate_eqns in H.
+    simpl in H.
+    apply stmt_eval_fold_left_shift in H.
+    destruct H as [menv'' H].
+    destruct H as [env'' H].
+    exists menv''. exists env''.
+    destruct H as [H1 H2].
+    split. apply H1.
+    inversion_clear H2.
+    inversion H0.
+    rewrite <- H2.
+    rewrite <- H4.
+    apply H.
+  - intro H.
+    destruct H as [menv'' H].
+    destruct H as [env'' H].
+    destruct H as [H1 H2].
+    unfold translate_eqns.
+    simpl.
+    apply stmt_eval_fold_left_shift.
+    exists menv''. exists env''.
+    split. apply H1.
+    eapply Icomp. apply H2.
+    apply Iskip.
+Qed.
+
 
 Lemma stmt_eval_Control:
   forall menv env mems c s menv' env',
@@ -386,443 +393,6 @@ Proof.
     reflexivity.
 Qed.
 
-Inductive sem_held_equation (H: history) (H': history) : equation -> Prop :=
-| SHEqDef:
-    forall x cae,
-      (forall n c, sem_var H x n (present c) -> sem_var H' x n (present c))
-      -> sem_held_equation H H' (EqDef x cae)
-| SHEqApp:
-    forall x f lae,
-      (forall n c, sem_var H x n (present c) -> sem_var H' x n (present c))
-      -> sem_held_equation H H' (EqApp x f lae)
-| SHEqFby:
-    forall x v0 lae ys,
-      (forall n, sem_laexp H lae n (ys n))
-      -> (forall n c, sem_var H' x n (present c) <-> holdR v0 ys n c)
-      -> sem_held_equation H H' (EqFby x v0 lae).
-
-Definition sem_held_equations
-           (H: history) (H': history) (eqs: list equation) : Prop :=
-  List.Forall (sem_held_equation H H') eqs.
-
-Lemma sem_held_equations_tl:
-  forall H H' eq eqs,
-    sem_held_equations H H' (eq::eqs) -> sem_held_equations H H' eqs.
-Proof.
-  intros H H' eq eqs Hsem.
-  apply Forall_cons2 in Hsem.
-  intuition.
-Qed.
-
-Lemma holdR_ext:
-  forall xs ys,
-    (forall n, xs n = ys n)
-    -> forall v0 n c,
-      holdR v0 xs n c
-      <-> holdR v0 ys n c.
-Proof.
-  intros xs ys Heq.
-  induction n.
-  - split; inversion 1; constructor.
-  - intro c.
-    split;
-    (inversion 1 as [|? ? Hv Hhold|? ? Hv];
-     (rewrite Heq in Hv || rewrite <- Heq in Hv);
-     [ apply IHn in Hhold; now constructor
-     | apply holdR_present with (1:=Hv) ]).
-Qed.
-
-Lemma fbyR_holdR:
-  forall v0 xs n c,
-    fbyR v0 xs n (present c)
-    -> holdR v0 xs n c.
-Proof.
-  inversion 1; intuition.
-Qed.
-
-Lemma sem_held_equations_corres:
-  forall G H H' eqs,
-    sem_equations G H eqs
-    -> sem_held_equations H H' eqs
-    -> (forall x n c,
-           Is_defined_in x eqs
-           -> sem_var H x n (present c)
-           -> sem_var H' x n (present c)).
-Proof.
-  induction eqs as [|eq]; [inversion 3|].
-  intros Hs Hsh x n c Hdef Hsv.
-  apply Forall_cons2 in Hs; destruct Hs as [Hseq Hseqs];
-  apply Forall_cons2 in Hsh; destruct Hsh as [Hsheq Hsheqs];
-  apply Is_defined_in_cons in Hdef; destruct Hdef as [Hdef|Hdef];
-  [ | destruct Hdef as [Hndef Hdef];
-      apply (IHeqs Hseqs Hsheqs _ _ _ Hdef Hsv) ].
-  destruct eq as [| |y v0 lae]; inversion Hdef; subst;
-  inversion_clear Hsheq as [? ? HH|? ? ? HH|? ? ? ys Hys HH];
-  apply HH; try apply Hsv.
-
-  inversion_clear Hseq as [| |? xs ? ? Hxs Hfby].
-  assert (forall n, xs n = ys n) as Hxsys by
-        (intro n0;
-         specialize Hys with n0;
-         specialize Hxs with n0 (xs n0);
-         apply sem_laexp_det with H n0 lae;
-         (apply Hxs; reflexivity) || apply Hys).
-  apply Hfby in Hsv.
-  rewrite <- (holdR_ext _ _ Hxsys).
-  apply fbyR_holdR with (1:=Hsv).
-Qed.
-
-Section StreamGenerators.
-
-  Variable H: history.
-  Variable arbitrary : stream.
-
-  Definition const_eqb (c1: const) (c2: const) : bool :=
-    match (c1, c2) with
-    | (Cint z1, Cint z2) => BinInt.Z.eqb z1 z2
-    | (Cbool b1, Cbool b2) => Bool.eqb b1 b2
-    | _ => false
-    end.
-
-  Definition value_eqb (v1: value) (v2: value) : bool :=
-    match (v1, v2) with
-    | (present c1, present c2) => const_eqb c1 c2
-    | (absent, absent) => true
-    | _ => false
-    end.
-
-  Fixpoint str_clock (ck: clock) (n: nat) : bool :=
-    match ck with
-    | Cbase => true
-    | Con ck' x c => match PM.find x H with
-                     | None => false
-                     | Some xs => andb (str_clock ck' n)
-                                       (value_eqb (xs n) (present (Cbool c)))
-                     end
-    end.
-
-  Fixpoint str_lexp (e: lexp) (n: nat) : value :=
-    match e with
-    | Econst c => present c
-    | Evar x => match PM.find x H with
-                | Some xs => xs n
-                | None => absent
-                end
-    | Ewhen e' x c => match PM.find x H with
-                      | Some xs => match xs n with
-                                   | present (Cbool b) =>
-                                     if Bool.eqb b c
-                                     then str_laexp e' n
-                                     else absent
-                                   | _ => absent
-                                   end
-                      | None => absent
-                      end
-    end
-  with str_laexp (e: laexp) (n: nat) : value :=
-    match e with
-    | LAexp ck e => if str_clock ck n then str_lexp e n else absent
-    end.
-
-  Lemma str_clock_spec:
-    forall ck n c,
-      sem_clock H ck n c
-      -> str_clock ck n = c.
-  Proof.
-    induction ck.
-    inversion 1; intuition.
-    intros n c.
-    inversion_clear 1;
-      repeat progress (simpl;
-         match goal with
-         | H:sem_var _ _ _ _ |- _ => inversion_clear H
-         | H: PM.find _ _ = _ |- _ => rewrite H
-         | H: _ = present (Cbool ?b) |- _ => (rewrite H; destruct b)
-         | H: sem_clock _ _ _ _ |- _ => (apply IHck in H; rewrite H)
-         | H: b <> _ |- _ => (apply Bool.not_true_is_false in H
-                              || apply Bool.not_false_is_true in H;
-                              rewrite H)
-         | _ => (cbv; reflexivity)
-         end).
-    destruct (PM.find i H); cbv; reflexivity.
-  Qed.
-
-  Lemma str_lexp_spec:
-    forall e n v,
-      sem_lexp H e n v
-      -> str_lexp e n = v.
-  Proof.
-    induction e using lexp_mult
-    with (P:=fun e => forall n v, sem_laexp H e n v -> str_laexp e n = v);
-    inversion 1;
-    repeat progress (simpl;
-           match goal with
-           | H:sem_lexp _ _ _ _ |- _ => (apply IHe in H; rewrite H)
-           | H:sem_laexp _ _ _ _ |- _ => (apply IHe in H; rewrite H)
-           | H:sem_clock _ _ _ _ |- _ => (apply str_clock_spec in H; rewrite H)
-           | H:sem_var _ _ _ _ |- _ => (inversion_clear H as [xs Hfind Hxsn];
-                                        rewrite Hfind; rewrite Hxsn)
-           | |- (if Bool.eqb ?b1 ?b2 then _ else _) = _ =>
-             try destruct b1; try destruct b2; simpl; intuition
-           | _ => intuition
-           end).
-  Qed.
-
-  Lemma str_laexp_spec:
-    forall e n v,
-      sem_laexp H e n v
-      -> str_laexp e n = v.
-  Proof.
-    inversion_clear 1; simpl;
-    repeat progress
-           match goal with
-           | H:sem_clock _ _ _ _ |- _ => (apply str_clock_spec in H; rewrite H)
-           | H:sem_lexp _ _ _ _ |- _ => (apply str_lexp_spec in H; rewrite H)
-           | _ => intuition
-           end.
-  Qed.
-
-End StreamGenerators.
-
-Definition hold_history (H: history) : history -> list equation -> history :=
-  List.fold_right
-    (fun eq H' =>
-       match eq with
-       | EqFby x v0 e => PM.add x (fun n=>present (hold v0 (str_laexp H e) n)) H'
-       | EqApp x _ _ => H'
-       | EqDef x _ => H'
-       end).
-
-Lemma hold_injection:
-  forall xs ys c n,
-    (forall n, xs n = ys n)
-    -> hold c xs n = hold c ys n.
-Proof.
-  intros xs ys c n Heq.
-  induction n.
-  auto.
-  case_eq (xs n).
-  intro Habs.
-  assert (ys n = absent) as Habs' by (rewrite Heq in Habs; intuition).
-  unfold hold.
-  rewrite Habs. rewrite Habs'.
-  fold hold.
-  apply IHn.
-
-  intros v Habs.
-  assert (ys n = present v) as Habs' by (rewrite Heq in Habs; intuition).
-  unfold hold.
-  rewrite Habs. rewrite Habs'.
-  reflexivity.
-Qed.
-
-Lemma Some_injection:
-  forall A (x:A) (y:A), x = y <-> Some x = Some y.
-Proof.
-  split; intro H; [rewrite H|injection H]; auto.
-Qed.
-
-Lemma present_injection:
-  forall x y, x = y <-> present x = present y.
-Proof.
-  split; intro H; [rewrite H|injection H]; auto.
-Qed.
-
-Lemma sem_var_gso:
-  forall x y xs n v H,
-    x <> y
-    -> (sem_var (PM.add x xs H) y n v <-> sem_var H y n v).
-Proof.
-  split; inversion_clear 1;
-  repeat progress match goal with
-                  | H:?xs _ = _ |- _ => apply Sv with xs
-                  | H:PM.find _ _ = Some _ |- _ => rewrite <- H
-                  | |- context [PM.find _ (PM.add _ _ _)] => rewrite PM.gso
-                  end; intuition.
-Qed.
-
-(* An alternative lemma would be:
-   sem_held_equations H H' (filter_dup_defs eqs) -> sem_held_equations H H' eqs
-   which should hold since the H in sem_equations/sem_held_equations requires
-   that multiple definitions of the same variable be coherent. But proving
-   this stronger result is much harder than just assuming something that
-   should anyway be true: there are no duplicate definitions in eqs.
-
-   Note, however, that this requires a stronger definition of Is_well_sch. *)
-Lemma not_in_add_to_sem_held_equations:
-  forall x xs eqs H H',
-    ~Is_defined_in x eqs
-    -> sem_held_equations H H' eqs
-    -> sem_held_equations H (PM.add x xs H') eqs.
-Proof.
-  induction eqs as [|eq].
-  intuition (apply List.Forall_nil).
-  intros H H' Hndef Hsem.
-  apply not_Is_defined_in_cons in Hndef; destruct Hndef as [Hndef0 Hndef1].
-  unfold sem_held_equations in Hsem.
-  apply Forall_cons2 in Hsem; destruct Hsem as [Hsem0 Hsem1].
-  apply (IHeqs _ _ Hndef1) in Hsem1.
-  destruct eq; [ apply not_Is_defined_in_eq_EqDef in Hndef0
-               | apply not_Is_defined_in_eq_EqApp in Hndef0
-               | apply not_Is_defined_in_eq_EqFby in Hndef0 ];
-  apply List.Forall_cons; try apply Hsem1;
-  inversion_clear Hsem0 as [? ? Hsv|? ? ? Hsv|? ? ? ys Hlae Hsv];
-  try constructor;
-  intros;
-  try (apply sem_var_gso with (1:=Hndef0); apply Hsv; assumption).
-  apply SHEqFby with (1:=Hlae).
-  intros; rewrite <- Hsv; split; intro HH.
-  apply sem_var_gso with (1:=Hndef0) in HH; assumption.
-  apply sem_var_gso with (1:=Hndef0); assumption.
-Qed.
-
-Inductive no_dup_defs : list equation -> Prop :=
-| NoDupDefs_nil : no_dup_defs nil
-| NoDupDefs_cons : forall eq eqs,
-                     (forall x, Is_defined_in_eq x eq
-                                -> ~Is_defined_in x eqs)
-                     -> no_dup_defs eqs
-                     -> no_dup_defs (eq::eqs).
-
-(*
-   eqs = [ EqDef x y; EqFby y (Cint 0) (Econst (Cint 1)) ]
-   eqs' = eqFby x (Cint 0) (Econst (Cint 1)) :: eqs
-
-   Both eqs and eqs' have a coherent semantics (sem_equations G H _),
-   but their respective hold semantics differ (for eqs', x is always present).
-*)
-Lemma sem_held_equations_existence:
-  forall G H eqs,
-    sem_equations G H eqs
-    -> no_dup_defs eqs
-    -> sem_held_equations H (hold_history H H eqs) eqs
-       /\ (forall y n c,
-              sem_var H y n (present c)
-              -> sem_var (hold_history H H eqs) y n (present c)).
-Proof.
-  intros G H eqs Hsem Hndups.
-  induction eqs as [|eq].
-  - intuition constructor.
-  - apply Forall_cons2 in Hsem; destruct Hsem as [Hsem Hsems].
-    apply IHeqs in Hsems; [clear IHeqs
-                          | inversion_clear Hndups; assumption ].
-    destruct Hsems as [Hsems Hvars].
-    destruct eq.
-
-    split; [apply Forall_cons2|intuition];
-    split; [constructor; apply Hvars|intuition].
-
-    split; [apply Forall_cons2|intuition];
-    split; [constructor; apply Hvars|intuition].
-
-    split.
-
-    (* show: sem_var -> sem_var *)
-    Focus 2.
-    intros y n c0 Hvar.
-    pose proof (Hvars _ _ _ Hvar) as Hvar'.
-    destruct (ident_eq_dec i y) as [Hiy|Hniy]; [rewrite Hiy|].
-    2:(inversion_clear Hvar'; apply Sv with xs; simpl; try rewrite PM.gso; auto).
-    simpl.
-    eapply Sv.
-    rewrite PM.gss.
-    rewrite <-Some_injection.
-    reflexivity.
-    simpl.
-    apply present_injection.
-    inversion_clear Hsem.
-    rewrite Hiy in *.
-    apply H1 in Hvar.
-    rewrite hold_injection with _ xs _ _.
-    apply hold_rel.
-    apply fbyR_holdR.
-    exact Hvar.
-    intro n0.
-    specialize H0 with n0 (xs n0).
-    assert (sem_laexp H l n0 (xs n0)) as Hsl by (apply H0; reflexivity).
-    apply str_laexp_spec in Hsl.
-    exact Hsl.
-
-    (* show sem_held_equations *)
-
-    simpl.
-    apply Forall_cons2.
-    split.
-    inversion_clear Hsem.
-    apply SHEqFby with xs.
-    intro n; apply H0 with (v:=xs n); reflexivity.
-    intros n c0.
-    split.
-    inversion_clear 1.
-    rewrite PM.gss in H3.
-    injection H3.
-    intro.
-    rewrite <-H2 in H4.
-    injection H4.
-    intro.
-    apply hold_rel.
-    rewrite <-H5.
-    apply hold_injection.
-    intro n0.
-    specialize H0 with n0 (xs n0).
-    assert (xs n0 = xs n0) as Hlae by reflexivity.
-    apply H0 in Hlae.
-    apply str_laexp_spec in Hlae.
-    rewrite Hlae.
-    reflexivity.
-    intro Hhold.
-    apply hold_rel in Hhold.
-    eapply Sv.
-    rewrite PM.gss.
-    rewrite <-Some_injection.
-    reflexivity.
-    simpl.
-    apply present_injection.
-    rewrite hold_injection with _ xs _ _.
-    apply Hhold.
-    intro n0.
-    specialize H0 with n0 (xs n0).
-    assert (sem_laexp H l n0 (xs n0)) as Hsl by (apply H0; reflexivity).
-    apply str_laexp_spec in Hsl.
-    exact Hsl.
-
-    apply not_in_add_to_sem_held_equations.
-    inversion_clear Hndups as [|? ? Hndups'].
-    apply Hndups'.
-    constructor.
-    apply Hsems.
-Qed.
-
-Lemma sem_held_equations_exist:
-  forall G H eqs,
-    sem_equations G H eqs
-    -> no_dup_defs eqs
-    -> exists H', sem_held_equations H H' eqs.
-Proof.
-  intros H H' eqs Hsems Hndups.
-  apply sem_held_equations_existence in Hsems.
-  destruct Hsems as [Hsems].
-  now (eexists; apply Hsems).
-  assumption.
-Qed.
-
-(* TODO: Is there a more direct way to negate PS.mem_spec?
-         I.e., without creating a distinct lemma. *)
-Lemma mem_spec_false:
-  forall s x, PS.mem x s = false <-> ~PS.In x s.
-Proof.
-  split.
-  intros Hmem Hin.
-  apply PS.mem_spec in Hin.
-  rewrite Hin in Hmem.
-  discriminate.
-  intro Hnin.
-  apply Bool.not_true_iff_false.
-  intro Hnmem.
-  rewrite PS.mem_spec in Hnmem.
-  contradiction.
-Qed.
-
 Local Ltac split_env_assumption :=
   match goal with
   | Henv: context Is_free_in_lexp [_], Hsem: sem_var _ ?y _ _
@@ -830,21 +400,6 @@ Local Ltac split_env_assumption :=
   | Henv: context Is_free_in_clock [_], Hsem: sem_var _ ?y _ _
     |- _ => apply Henv in Hsem; [destruct Hsem |solve [auto]]; clear Henv
   end.
-
-Lemma exp_eval_tovar:
-  forall x v menv env memories,
-    exp_eval menv env (tovar memories x) v
-    <-> (exp_eval menv env (State x) v /\ PS.In x memories)
-        \/ (exp_eval menv env (Var x) v /\ ~PS.In x memories).
-Proof.
-  split; intro Heval;
-  destruct In_dec with x memories as [Hxm|Hxm];
-    pose proof Hxm as Hxmt;
-    apply PS.mem_spec in Hxmt || apply mem_spec_false in Hxmt;
-    unfold tovar in *;
-    rewrite Hxmt in *;
-    intuition.
-Qed.
 
 (* Note that the converse:
        Is_present_in memories menv env ck -> sem_clock H ck n true
@@ -1113,88 +668,6 @@ Local Ltac resolve_env_assumption :=
 
 Import List.ListNotations.
 Open Scope list_scope.
-
-Lemma List_shift_first:
-  forall (A:Set) ll (x : A) lr,
-    ll ++ (x :: lr) = (ll ++ [x]) ++ lr.
-Proof.
-  induction ll as [|? ? IH]; [auto|intros].
-  rewrite <- List.app_comm_cons.
-  rewrite IH.
-  now do 2 rewrite List.app_comm_cons.
-Qed.
-
-Lemma List_shift_away:
-  forall (A:Set) alleqs (eq : A) eqs,
-    (exists oeqs, alleqs = oeqs ++ (eq :: eqs))
-    -> exists oeqs', alleqs = oeqs' ++ eqs.
-Proof.
-  intros A alleqs eq eqs Hall.
-  destruct Hall as [oeqs Hall].
-  exists (oeqs ++ [eq]).
-  rewrite Hall.
-  now rewrite List_shift_first.
-Qed.
-
-Lemma Forall_app:
-  forall A (P: A -> Prop) ll rr,
-    List.Forall P (ll ++ rr) <-> (List.Forall P ll /\ List.Forall P rr).
-Proof.
-  intros A P ll rr.
-  induction ll as [|x ll IH]; [intuition|].
-  rewrite Forall_cons2.
-  rewrite and_assoc.
-  rewrite <-IH.
-  rewrite <-List.app_comm_cons.
-  now rewrite Forall_cons2.
-Qed.
-
-Lemma sem_equations_app2:
-  forall G H oeqs eqs,
-    sem_equations G H (oeqs ++ eqs)
-    -> sem_equations G H eqs.
-Proof.
-  intros G H oeqs eqs H0.
-  apply Forall_app in H0; intuition.
-Qed.
-
-Lemma sem_held_equations_app2:
-  forall H H' oeqs eqs,
-    sem_held_equations H H' (oeqs ++ eqs)
-    -> sem_held_equations H H' eqs.
-Proof.
-  intros H H' oeqs eqs H0.
-  apply Forall_app in H0; intuition.
-Qed.
-
-Lemma sem_held_equations_cons:
-  forall H H' eq eqs,
-    sem_held_equations H H' (eq :: eqs)
-    <-> sem_held_equation H H' eq /\ sem_held_equations H H' eqs.
-Proof.
-  split; intro Hs.
-  apply Forall_cons2 in Hs; auto.
-  apply Forall_cons2; auto.
-Qed.
-
-Lemma find_mem_gss:
-  forall y c m, find_mem y (add_mem y c m) = Some c.
-Proof.
-  intros. apply PM.gss.
-Qed.
-
-Lemma find_mem_gso:
-  forall x y c m, x <> y -> find_mem x (add_mem y c m) = find_mem x m.
-Proof.
-  intros. apply PM.gso. assumption.
-Qed.
-
-Lemma Is_memory_in_EqFby:
-  forall y v0 lae eqs,
-    Is_memory_in y (EqFby y v0 lae :: eqs).
-Proof.
-  intros. repeat constructor.
-Qed.
 
 Lemma is_step_correct:
   forall (G: global)
