Common.v
@@ -25,3 +25,74 @@ Lemma Forall_cons2:
     List.Forall P (x :: l) <-> P x /\ List.Forall P l.
 Proof. intros; split; inversion_clear 1; auto. Qed.
 
+Lemma pm_in_dec: forall A i m, PM.In (A:=A) i m \/ ~PM.In (A:=A) i m.
+Proof.
+  unfold PM.In, PM.MapsTo.
+  intros A i m.
+  case (PM.find i m).
+  eauto.
+  right; intro; destruct H; discriminate H.
+Qed.
+
+Lemma Some_injection:
+  forall A (x:A) (y:A), x = y <-> Some x = Some y.
+Proof.
+  split; intro H; [rewrite H|injection H]; auto.
+Qed.
+
+(* TODO: Is there a more direct way to negate PS.mem_spec?
+         I.e., without creating a distinct lemma. *)
+Lemma mem_spec_false:
+  forall s x, PS.mem x s = false <-> ~PS.In x s.
+Proof.
+  split.
+  intros Hmem Hin.
+  apply PS.mem_spec in Hin.
+  rewrite Hin in Hmem.
+  discriminate.
+  intro Hnin.
+  apply Bool.not_true_iff_false.
+  intro Hnmem.
+  rewrite PS.mem_spec in Hnmem.
+  contradiction.
+Qed.
+
+Import List.ListNotations.
+Open Scope list_scope.
+
+Lemma List_shift_first:
+  forall (A:Set) ll (x : A) lr,
+    ll ++ (x :: lr) = (ll ++ [x]) ++ lr.
+Proof.
+  induction ll as [|? ? IH]; [auto|intros].
+  rewrite <- List.app_comm_cons.
+  rewrite IH.
+  now do 2 rewrite List.app_comm_cons.
+Qed.
+
+Lemma List_shift_away:
+  forall (A:Set) alleqs (eq : A) eqs,
+    (exists oeqs, alleqs = oeqs ++ (eq :: eqs))
+    -> exists oeqs', alleqs = oeqs' ++ eqs.
+Proof.
+  intros A alleqs eq eqs Hall.
+  destruct Hall as [oeqs Hall].
+  exists (oeqs ++ [eq]).
+  rewrite Hall.
+  now rewrite List_shift_first.
+Qed.
+
+Lemma Forall_app:
+  forall A (P: A -> Prop) ll rr,
+    List.Forall P (ll ++ rr) <-> (List.Forall P ll /\ List.Forall P rr).
+Proof.
+  intros A P ll rr.
+  induction ll as [|x ll IH]; [intuition|].
+  rewrite Forall_cons2.
+  rewrite and_assoc.
+  rewrite <-IH.
+  rewrite <-List.app_comm_cons.
+  now rewrite Forall_cons2.
+Qed.
+
+
